\documentclass[14pt]{article}
\usepackage{amsmath}

\newcommand{\slashed}[1]{\hbox{{$#1$}\llap{$/$}}}
\begin{document}

\begin{center}
	{\Large\bf\underline{The Table of Integrals and Formulae}}
\end{center}

\bigskip

\begin{eqnarray}
\nonumber
&&	\int \frac{d^4k}{(2\pi)^4} 
		\frac{1}{k^4} =
		\frac{i}{8 \pi^2} \log \Lambda/\mu   \\
\nonumber
&&	\int \frac{d^4k}{(2\pi)^4} 
		\frac{1}{k^2} =
		-i \frac{1}{16\pi^2}\Lambda^2		\\
\nonumber
&&	\int \frac{d^4k}{(2\pi)^4} 
		\frac{k^\mu k^\nu} 
		     {k^2 (p - k)^2} =
		-\frac{i}{64\pi^2}g^{\mu\nu}\Lambda^2 +
		\frac{i}{24\pi^2}
		\left(p^\mu p^\nu - \frac{1}{4}p^2 g^{\mu\nu}\right)
		\log \Lambda/\mu 			\\
\nonumber
&&	\int \frac{d^4k}{(2\pi)^4} 
		\frac{k^\alpha}
		     {k^2 (p - k)^2} =
		\frac{i}{16\pi^2}p^\alpha \log \Lambda/\mu 	\\
\nonumber
&&	\int \frac{d^4k}{(2\pi)^4} 
		\frac{k^\mu (k^\nu - p^\nu)}
		     {k^2 (p - k)^2} =
		-\frac{i}{64\pi^2}g^{\mu\nu}\Lambda^2 -
		\frac{i}{48\pi^2}\left(p^\mu p^\nu + 
				       \frac{1}{2}g^{\mu\nu}p^2\right)
					\log \Lambda/\mu	\\
\nonumber
&&	\int \frac{d^4k}{(2\pi)^4} 
		\frac{k^\mu (k^\nu + p^\nu)}
		     {k^2 (p - k)^2} =
		-\frac{i}{64\pi^2}g^{\mu\nu}\Lambda^2 +
		i\frac{5}{48\pi^2}\left(p^\mu p^\nu -
				       \frac{1}{2}g^{\mu\nu}p^2\right)
					\log \Lambda/\mu	\\
\nonumber
&&	\int \frac{d^4k}{(2\pi)^4} 
		\frac{k^\alpha k^\beta k^\gamma k^\delta}
		     {k^4 (p - k)^2} =
		- \frac{i}{384\pi^2}
		\left(g^{\alpha\beta}g^{\gamma\delta} +
		      g^{\alpha\gamma}g^{\beta\delta} +
                      g^{\alpha\delta}g^{\beta\gamma}\right)
		\left(\Lambda^2 + p^2 \log \Lambda/\mu\right) + \\
\nonumber
&&~~~~~~~~~~~~~~~~~~~~~~~~~~~~~~~~
		\frac{i}{192\pi^2}
		\Bigl(p^{\alpha}p^{\beta}g^{\gamma\delta} +
		      p^{\alpha}p^{\gamma}g^{\beta\delta} +
		      p^{\alpha}p^{\delta}g^{\beta\gamma} +     \\
\nonumber
&&~~~~~~~~~~~~~~~~~~~~~~~~~~~~~~~~~~~~~~~~~~
		      p^{\gamma}p^{\delta}g^{\alpha\beta} +
		      p^{\beta}p^{\delta}g^{\alpha\gamma} +
		      p^{\beta}p^{\gamma}g^{\alpha\delta}\Bigr)
		\log \Lambda/\mu \\
\nonumber
&&	\int \frac{d^4k}{(2\pi)^4} 
	     \frac{(p + k)^2}
		  {k^2 (p - k)^2} =
	    - \frac{i}{16\pi^2} \Lambda^2  +
    		\frac{i}{4 \pi^2} p^2 \log \Lambda/\mu   \\
\nonumber
&&
\parbox{7.0cm}
{
$$
	\frac{1}
	     {k^2 (p - k)^2}  = 
		\int_0^1
		\frac{dx}
		     {(q^2 + xy p^2)^2}~   
$$
$$
	\frac{1}
	     {k^4 (p - k)^2}  = 
		\int_0^1
		\frac{2 x dx}
		     {(q^2 + xy p^2)^3}~  
$$
}
\hspace{1.7cm}
	\parbox{3.0cm}{
		\begin{tabular}{l}
			$ q \equiv k - yp~, $ \\
	          	$ k = q + yp~,~$ \\
		      	$ y \equiv 1 - x $ \\
		\end{tabular}
			}
\end{eqnarray}


\newpage


\begin{eqnarray}
&&\nonumber
   B(\alpha,\beta) = \int_0^1 x^{\alpha-1}(1 - x)^{\beta - 1} dx = 
		\frac {\Gamma(\alpha)\Gamma(\beta)}
                      {\Gamma(\alpha + \beta)}       \\
&&\nonumber
	\int_0^1 dx ~... = \int_0^1 dy ...~,\hspace{2.0cm} y = 1 - x \\
&&\nonumber
	k^\mu k^\nu~~ \to~~ \frac{1}{4} k^2 g^{\mu\nu}  \hspace{9.0cm}\\
&&\nonumber
	k^\alpha k^\beta k^\gamma k^\delta ~~\to~~  
	\frac{1}{24}k^4 
		\left(g^{\alpha\beta}g^{\gamma\delta} +
		      g^{\alpha\gamma}g^{\beta\delta} +
                      g^{\alpha\delta}g^{\beta\gamma}\right) \\
&&\nonumber
	\text{The volume of the 3-d sphere is $ 2\pi^2 $}
\end{eqnarray}

\begin{eqnarray}
&&\nonumber
	C^{\alpha\beta\gamma}\gamma_\alpha \gamma_\rho \gamma_\beta =
	2 C^{\rho\gamma\alpha}\gamma_\alpha - 
	C^{\alpha\alpha\gamma}\gamma^\rho \hspace{7.0cm}  \\
&&\nonumber
	C^{\alpha\beta\gamma}\gamma_\alpha \gamma_\beta \gamma_\gamma =
	C^{\alpha\alpha\beta}\gamma_\beta
\end{eqnarray}

\begin{tabular}{ll}
{\it Chiral representation} of $\gamma$-matrices: &
$
	\gamma^0 = \left[
	\begin{array}{cc}
	        &   1 \\
            1   &
	\end{array}\right],~~
	\gamma^i = \left[
	\begin{array}{cc}
	        &   \sigma^i \\
            -\sigma^i   &
	\end{array}\right],~~
	\gamma^5 = \left[
	\begin{array}{cc}
	    -1  &    \\
                &  1
	\end{array}\right]
$ \\
{\it Standard representation} of $\gamma$-matrices: &
$
	\gamma^0 = \left[
	\begin{array}{cc}
	    1   &     \\
                &   -1
	\end{array}\right],~~
	\gamma^i = \left[
	\begin{array}{cc}
	        &   \sigma^i \\
            -\sigma^i   &
	\end{array}\right]
$ \\
We use the {\bf standard representation} &\\
$~~~~~~~~~~\gamma^5 = i \gamma^0 \gamma^1 \gamma^2 \gamma^3 =
	\left[
	\begin{array}{cc}
	     0  &  1  \\
             1  &  0
	\end{array}\right] $

\end{tabular}

\vspace{1.0cm}
\parbox{8.0cm}{
\begin{eqnarray*}
 && {\rm Tr} \left (\gamma^\mu \gamma^\nu \right)  = 4 g^{\mu\nu} \\
 && {\rm Tr} \left (\gamma^\mu \gamma^\nu \gamma^\rho \gamma^\sigma 
		   \gamma^5 \right) = - 4 i \epsilon^{\mu\nu\rho\sigma} \\
 && {\rm Tr} \left (\gamma^\alpha \gamma^\beta \gamma^\gamma \gamma^\delta
		\right) =
	4\left(g^{\alpha\beta}g^{\gamma\delta} -
		g^{\alpha\gamma}g^{\beta\delta} +
                g^{\alpha\delta}g^{\beta\gamma}\right) \\
 &&  \gamma^\alpha \gamma^\beta \gamma^\gamma = 
	g^{\alpha\beta}\gamma^\gamma + g^{\beta\gamma}\gamma^\alpha -
	g^{\alpha\gamma}\gamma^\beta - 
	i \epsilon^{\alpha\beta\gamma\delta} \gamma^5\gamma^\delta
\end{eqnarray*}
\begin{eqnarray*}
  \gamma^\mu \gamma^\alpha \gamma^\beta \gamma^\gamma \gamma_\mu & = &
	-2 \gamma^\gamma \gamma^\beta \gamma^\alpha \\
  \gamma^\mu \gamma^\alpha \gamma^\beta \gamma_\mu & = &
	4 g^{\alpha\beta} \\
  \gamma^\mu \gamma^\alpha \gamma_\mu & = &
	- 2 \gamma^\alpha \\
  \gamma^\mu \gamma_\mu & = & 4
\end{eqnarray*}
}
\parbox[b]{5.0cm}
{
\begin{eqnarray*}
&& \epsilon_{\mu\alpha\beta\gamma} \gamma^\alpha \gamma^\beta \gamma^\gamma =
		- 6 i \gamma^5 \gamma_\mu \\
&& \epsilon^{\alpha\beta\gamma\delta}\epsilon_{\alpha\beta\gamma\sigma} =
	 -6 \delta^\delta_\sigma \\
&& \epsilon^{\alpha\beta\gamma\delta}\epsilon_{\alpha\beta\mu\nu} = 
	 -2 \left [ \delta_\mu^\gamma \delta_\nu^\delta - 
		    \delta_\nu^\gamma \delta_\mu^\delta \right ] 
\end{eqnarray*}
}

\parbox{5.0cm}
{
\begin{eqnarray*}
&&	\left[ \sigma^a \sigma^b \right] = 2 i \epsilon^{abc} \sigma^c \\
&&	\left[ \tau^a \tau^b \right] = i \epsilon^{abc} \tau^c 
\end{eqnarray*}
}
\parbox{5.0cm}
{
\begin{equation*}
	\tau^a \equiv \frac{1}{2} \sigma^a
\end{equation*}
}
\parbox{5.0cm}
{
\begin{eqnarray*}
	\left\{ \sigma^a \sigma^b \right\} = 2 \delta^{ab} &&\\
	\left\{ \tau^a \tau^b \right\} = \frac{1}{2} \delta^{ab} &&
\end{eqnarray*}
}

\[
~~~~~{\rm Tr} \left( T^a T^b \right) \equiv \frac{1}{2}\delta^{ab},~~~~~~~~~~~
T^a T^b = 1_{fund} \cdot \frac{ N^2 - 1} {2 N},~~~~~~~~~~~
f^{abc}f^{dbc} = N\cdot \delta^{ad}
\]

\[
F_{\mu\nu}F^{\mu\nu} = - 2 A^\mu\left ( \partial^2 g^{\mu\nu} -
					\partial_\mu\partial_\nu \right) A^\nu
\]


1-loop QED renormalization constants
\[
   Z_\psi = 1 - \frac{e^2}{8\pi^2}\log\Lambda/\mu,~~~~~
   Z_e = 1 - \frac{e^2}{8\pi^2}\log\Lambda/\mu,~~~~~
   Z_A = 1 - \frac{e^2}{6\pi^2}\log\Lambda/\mu
\]

\renewcommand{\arraystretch}{1.5}
\begin{tabular}{|c|c|}
\hline
\multicolumn{2}{|c|}{\it LV Operators in the Standard Model} \\
\hline
\hline
 & Feynman rules  \\
\raisebox{2.2ex}[0pt]{Operator} & (assuming $p$ incoming) \\
\hline
\hline
$
C^{\alpha\beta\gamma}\bar{Q}\eta_Q
\partial^\alpha\partial^\beta\partial^\gamma P_L Q 
$ &
$
- i \eta_Q^{\rm fl} C^{\alpha\beta\gamma} p^\alpha p^\beta \gamma^\gamma
			P_L \delta^{\rm isospin}
$  \\

$ C^{\alpha\beta\gamma}\bar{u}\eta_u
\partial^\alpha\partial^\beta\partial^\gamma P_R u
$ &
$
- i \eta_u^{\rm fl} C^{\alpha\beta\gamma} p^\alpha p^\beta \gamma^\gamma
			P_R 
$  \\

$ \xi_{\rm EM} A_\mu C^{\alpha\beta\gamma} 
  \epsilon^{\gamma\mu\nu\lambda} 
\partial_\alpha \partial_\beta \partial_\lambda A_\nu $ & 

$ 2 \xi_{\rm EM} C^{\alpha\beta\gamma}   \epsilon^{\gamma\mu\nu\lambda} 
	p_\alpha p_\beta p_\lambda $ \\

$ \xi' B_\mu C^{\alpha\beta\gamma} 
  \epsilon^{\gamma\mu\nu\lambda} 
\partial_\alpha \partial_\beta \partial_\lambda B_\nu $ & 

$ 2 \xi' C^{\alpha\beta\gamma}   \epsilon^{\gamma\mu\nu\lambda} 
	p_\alpha p_\beta p_\lambda $ \\

$ \xi W_\mu^a C^{\alpha\beta\gamma} 
  \epsilon^{\gamma\mu\nu\lambda} 
\partial_\alpha \partial_\beta \partial_\lambda W_\nu^a $ & 

$ 2 \xi C^{\alpha\beta\gamma}   \epsilon^{\gamma\mu\nu\lambda} 
	p_\alpha p_\beta p_\lambda \delta^{ab}$ \\

$ \xi_3 G_\mu^a C^{\alpha\beta\gamma} 
  \epsilon^{\gamma\mu\nu\lambda} 
\partial_\alpha \partial_\beta \partial_\lambda G_\nu^a $ & 

$ 2 \xi_3 C^{\alpha\beta\gamma}   \epsilon^{\gamma\mu\nu\lambda} 
	p_\alpha p_\beta p_\lambda \delta^{ab}$ \\

$ i \kappa H^\dag C^{\alpha\beta\gamma} 
\partial_\alpha \partial_\beta \partial_\gamma H $ &
$ -i \kappa C^{\alpha\beta\gamma} p_\alpha p_\beta p_\gamma 
	\delta^{\rm isospin} $ \\
\hline
\end{tabular}

\end{document}
